theories/νType/LeInductive.v
@@ -93,14 +93,12 @@ Proof.
   intros H1 H2. induction H1. now easy. now constructor.
 Defined.
 
-Lemma leI_invert : forall P : forall p n : nat, p <~ n -> Type,
-       (forall p : nat, P p p (leI_refl p)) ->
-       (forall (p n : nat) (l : p.+1 <~ n.+1),
-        P p.+1 n.+1 l -> P p n.+1 (leI_down l)) ->
-       forall (p n : nat) (l : p <~ n), P p n l.
+Lemma leI_invert {P : forall p n, p <~ n -> Type}
+  {Q: forall p, P p p (leI_refl p)}
+  {R: forall p n (l : p.+1 <~ n.+1), P p.+1 n.+1 l -> P p n.+1 (leI_down l)}
+  {p n} (l : p <~ n): P p n l.
 Proof.
-intros P H H0 p n.
 induction l.
-- apply H.
-- destruct n. destruct (leI_O_contra l). apply H0, IHl.
+- apply Q.
+- destruct n. destruct (leI_O_contra l). apply R, IHl.
 Defined.
